MPL/SProp.lean
@@ -1,4 +1,5 @@
 import MPL.SProp.SVal
 import MPL.SProp.SProp
 import MPL.SProp.Notation
-import MPL.SProp.Lemmas
+import MPL.SProp.Laws
+import MPL.SProp.DerivedLaws
