MPL/Triple.lean
@@ -9,93 +9,40 @@ def triple (x : m α) (P : PreCond ps) (Q : PostCond α ps) : Prop :=
   P ⊢ₛ wp⟦x⟧.apply Q
 
 syntax:lead "⦃" term "⦄ " term:lead " ⦃" term "⦄" : term
--- syntax:lead "⦃" term "⦄ " term:lead " ⦃⇓" ident " | " term "⦄" : term
-macro_rules
-  | `(⦃$P⦄ $x:term ⦃$Q⦄) => `(triple $x sprop($P) sprop($Q))
---  | `(⦃$P⦄ $x:term ⦃⇓ $v | $Q⦄) => `(triple $x sprop($P) (PostCond.total fun $v => sprop($Q)))
+open Lean Elab Meta Term
+elab_rules : term
+  | `(⦃$P⦄ $x:term ⦃$Q⦄) => do
+    -- In a simple world, this would just be a macro expanding to
+    -- `triple $x sprop($P) sprop($Q)`.
+    -- However, it appears that type inference for the
+    -- postcondition Q is better when implemented manually.
+    let x ← elabTerm x none
+    let ty ← inferType x
+    tryPostponeIfMVar ty
+    let .app m α := ty | throwError "Not a type application {ty}"
+    let some u ← Level.dec <$> getLevel ty | throwError "Wrong level 0 {ty}"
+    let ps ← mkFreshExprMVar (mkConst ``PredShape)
+    let inst ← synthInstance (mkApp2 (mkConst ``WP [u]) m ps)
+    let P ← elabTerm (← `(sprop($P))) (mkApp (mkConst ``PreCond) ps)
+    let Q ← elabTerm (← `(sprop($Q))) (mkApp2 (mkConst ``PostCond) α ps)
+    return mkApp7 (mkConst ``triple [u]) m ps inst α x P Q
 
 theorem triple_conseq {α} (x : m α) {P P' : PreCond ps} {Q Q' : PostCond α ps}
   (hp : P.entails P' := by simp) (hq : Q'.entails Q := by simp) (h : triple x P' Q') :
   triple x P Q := by
-    apply SProp.entails_trans hp
-    apply SProp.entails_trans h
+    apply SProp.entails.trans hp
+    apply SProp.entails.trans h
     apply wp⟦x⟧.mono Q' Q hq
 
-theorem triple_extract_persistent {α} {P : Prop} {P' : PreCond ps} {Q : PostCond α ps}
-  (x : m α) (h : P → triple x P' Q) :
-  triple (ps:=ps) x sprop(⌜P⌝ ∧ P') Q := PreCond.imp_pure_extract_l h
-
 theorem triple_pure [Monad m] [MonadMorphism m (PredTrans ps) wp] {α} {Q : PostCond α ps} (a : α) (himp : P.entails (Q.1 a)) :
-  triple (pure (f:=m) a) P Q := by apply SProp.entails_trans himp (by simp only [pure_pure, PredTrans.pure_apply, SProp.entails_refl])
+  triple (pure (f:=m) a) P Q := by apply SProp.entails.trans himp (by simp only [pure_pure, PredTrans.pure_apply, SProp.entails.refl])
 
 theorem triple_bind [Monad m] [MonadMorphism m (PredTrans ps) wp] {α β} {P : PreCond ps} {Q : α → PreCond ps} {R : PostCond β ps} (x : m α) (f : α → m β)
   (hx : triple x P (Q, R.2))
   (hf : ∀ b, triple (f b) (Q b) R) :
   triple (x >>= f) P R := by
-    apply SProp.entails_trans hx
+    apply SProp.entails.trans hx
     simp only [bind_bind]
     apply wp⟦x⟧.mono _ _
     simp only [PostCond.entails, PreCond, FailConds.entails_refl, and_true]
     exact hf
-
-/-
-theorem triple_bind2 [Monad m] [MonadMorphism m (PredTrans ps) wp] {α β} {P : PreCond ps} {R : PostCond β ps} (x : m α) (f : α → m β)
-  (h : triple x P (fun a => wp⟦f a⟧.apply R, R.2)) :
-  triple (x >>= f) P R := triple_bind x f h (fun _ => le_rfl)
--/
---theorem triple_bind_pre [Monad m] [MonadMorphism m (PredTrans ps) wp] {α β} {P : PreCond ps} {Q : PostCond β ps} (x : m α) (f : α → m β)
---  (hx : triple wp⟦x⟧ P (fun a => triple wp⟦f a⟧ Q, Q.2)) :
---  triple wp⟦x >>= f⟧ P R := by
---    apply le_trans hx
---    simp only [wp_bind]
---    apply wp_mono x
---    simp only [Prod.mk_le_mk, le_refl, and_true]
---    exact hf
-
-theorem triple_extract_persistent_true {α} (x : m α) {P : Prop} {Q : PostCond α ps}
-  (h : P → triple (ps:=ps) x ⌜True⌝ Q) :
-  triple x ⌜P⌝ Q := by
-    have : ⌜P⌝ = (sprop(⌜P⌝ ∧ ⌜True⌝) : PreCond ps) := by simp
-    rw[this]
-    exact triple_extract_persistent x h
-
-/-
-theorem triple_conseq_l [Monad m] [MonadMorphism m (PredTrans ps) wp] {P P' : PreCond ps} {Q : PostCond α ps}
-  (x : m α) (hp : P ≤ P') (h : triple x P' Q) :
-  triple x P Q := triple_conseq x hp le_rfl h
-
-theorem triple_conseq_r [Monad m] [MonadMorphism m (PredTrans ps) wp] {P : PreCond ps} {Q Q' : PostCond α ps}
-  (x : m α) (hq : Q ≤ Q') (h : triple x P Q) :
-  triple x P Q' := triple_conseq x le_rfl hq h
-
---theorem triple_map [Monad m] [LawfulMonad m] [MonadMorphism m (PredTrans ps) wp] (f : α → β) (x : m α)
---  (h : triple x P (fun a => Q.1 (f a), Q.2)) :
---  triple (f <$> x) P Q := by
---    simp only [← bind_pure_comp]
---    apply triple_bind _ _ h
---    intro b
---    apply triple_pure
---    simp only [le_refl]
-
---theorem triple_seq [Monad m] [LawfulMonad m] [MonadMorphism m (PredTrans ps) wp] (f : m (α → β)) (x : m α) {Q : (α → β) → PreCond ps}
---  (hf : triple f P (Q, R.2))
---  (hx : ∀ f, triple x (Q f) (fun a => R.1 (f a), R.2)) :
---  triple (f <*> x) P R := by
---    simp only [← bind_map]
---    apply triple_bind _ _ hf ?_
---    intro f
---    apply triple_map _ _ (hx f)
-
-theorem triple_dite {c : Prop} [Decidable c] {t : c → m α} {e : ¬c → m α} {P : PreCond ps} {Q : PostCond α ps} [Monad m] [WP m ps]
-  (htrue : (h : c) → triple (t h) P Q)
-  (hfalse : (h : ¬c) → triple (e h) P Q) :
-  triple (dite c t e) P Q := by
-    split <;> simp only [htrue, hfalse]
-
-theorem triple_ite {c : Prop} [Decidable c] {t : m α} {e : m α} {P : PreCond ps} {Q : PostCond α ps} [Monad m] [WP m ps]
-  (htrue : c → triple t P Q)
-  (hfalse : ¬c → triple e P Q) :
-  triple (ite c t e) P Q := by
-    change triple (dite c (fun _ => t) (fun _ => e)) P Q
-    exact triple_dite htrue hfalse
--/
